pulse/lib/pulse/core/PulseCore.Atomic.fst
@@ -286,7 +286,7 @@ let ghost_reveal (a:Type) (x:erased a)
 let dup_inv (i:iref) (p:slprop) = A.dup_inv i p
 
 let new_invariant (p:slprop3)
-: stt_ghost (i:iref{injective_iref i}) emp_inames p (fun i -> inv i p)
+: stt_ghost iref emp_inames p (fun i -> inv i p)
 = A.new_invariant p
 
 let fresh_invariant ctx p = A.fresh_invariant ctx p
@@ -311,7 +311,6 @@ let with_invariant_g #a #fp #fp' #f_opens #p i $f =
 let distinct_invariants_have_distinct_names i j _ =
   A.distinct_invariants_have_distinct_names i j ()
 let invariant_name_identifies_invariant p q i j =
-  assume (A.injective_iref j);
   A.invariant_name_identifies_invariant p q i j
 
 let pts_to_not_null #a #p r v = Ghost.hide (A.pts_to_not_null #a #p r v)
